---
aliases: [negation of predicates]
--- 

#logic 

## Facts 

> [!tldr] Facts
> Suppose $P(x)$ is a predicate. Then: 
> - The negation of its existentially quantified form $\exists x P(x)$ is $\forall x (\neg P(x))$. 
> - The negation of its universally quantified form $\forall x P(x)$ is $\exists x (\neg P(x))$. 
> 
> That is: $\neg (\exists x P(x)) = \forall x (\neg P(x))$ and $\neg (\forall x P(x)) = \exists x (\neg P(x))$. 

Notes: 
- In English, this is saying: 
	- The negation of "There exists an $x$ such that $P(x)$ is true", is the statement "For all $x$, $P(x)$ is false."
	- The negation of "For all $x$, $P(x)$ is true", is the statement "There exists an $x$ such that $P(x)$ is false."
- Note that in each case we not only negate the predicate, but change the quantifier. 

## Examples and Non-Examples

## Resources 

(video)

Other resources: 
- 

## Practice 
